Lista la definición de forces

src/Forces_Definition.thy
@@ -497,25 +497,6 @@ lemma arity_forces_mem_fm [simp]:
   done
 *)
 
-(*
-consts forces_ren :: "[i\<Rightarrow>i,i,i,i]\<Rightarrow>i"
-primrec
-  "forces_ren(auxren,fren,fref,Member(x,y)) = forces_mem_fm(x,y)" (* Not ready yet *)
-  "forces_ren(auxren,fren,fref,Equal(x,y))  = forces_eq_fm(auxren,x,y)"
-  "forces_ren(auxren,fren,fref,Nand(p,q))   = Forall(Forall(Implies(Member(1,2),
-                  Implies(And(pair_fm(1,5,0),Member(0,3)),
-                  Neg(And(fren`forces_ren(auxren,fren,fref,p), fren`forces_ren(auxren,fren,fref,q)))))))"
-  "forces_ren(auxren,fren,fref,Forall(p))   = Forall(fref`forces_ren(auxren,fren,fref,p))" (* check indexes *)
-
-*)
-
-(*
-consts forces_ren :: "i\<Rightarrow>i"
-primrec
-  "forces_ren(Member(x,y)) = forces_mem_fm(0,1,2,3,x#+4,y#+4)" (* Not ready yet *)
-  "forces_ren(Equal(x,y)) = forces_eq_fm(0,1,2,3,x#+4,y#+4)"
-*)
-
 context forcing_data
 begin
 
@@ -1053,216 +1034,100 @@ lemma sats_forces_mem_fm:
 end (* context forcing_data *)
 
 
-(*
-
-(* \<not>\<exists>q \<le> p. (forces(f) *)
+(* DEFINE THIS *)
 definition 
-  forces_neg :: "i\<Rightarrow>i" where
-  "forces_neg(f) \<equiv> Neg(Exists(And(leq_fm(2,0,4),forces(f))))"
+  ren_forces_nand :: "i\<Rightarrow>i" where
+  "ren_forces_nand(f) \<equiv> f" 
 
+lemma ren_forces_nand_type[TC] :
+  "\<phi>\<in>formula \<Longrightarrow> ren_forces_nand(\<phi>) \<in>formula" 
+  unfolding ren_forces_nand_def by simp
 
-
-Forall(f) 
-
-Forall(forces(f))
-
-env = [a , b,...,xx,....,yy,...]
-       0   5    ,
-
-[a',q,P,leq,one]@env'
-
-rand
-
-
-definition 
-  fleq_fm :: "[i,i,i,i] \<Rightarrow> i" where
-  "fleq_fm(qp,leq,q,p) \<equiv> And(pair_fm(q,p,qp),Member(qp,leq))" 
-
-consts forces :: "i\<Rightarrow>i"
-primrec
-  "forces(Member(x,y)) = forces_mem_fm(0,1,3,x#+4,y#+4)" (* Not ready yet *)
-  "forces(Equal(x,y))  = forces_eq_fm(0,1,3,x#+4,y#+4)"
-  "forces(Nand(p,q))   = Exists(Neg(Exists(And(leq_fm(0,3,1,5),r(And(forces(p),forces(q)))))))"
-
-    Forall(Forall(Implies(Member(1,2),
-                  Implies(And(pair_fm(1,5,0),Member(0,3)),
-                  Neg(And(fren`forces_ren(auxren,fren,fref,p), fren`forces_ren(auxren,fren,fref,q)))))))"
-  "forces_ren(auxren,fren,fref,Forall(p))   = Forall(fref`forces_ren(auxren,fren,fref,p))" (* check indexes *)
-
-
-
-
-
-(*
-lemma def_one: 
-  assumes 
-    "xa\<in>M"
-  shows 
-    "(\<forall>x\<in>M. x \<in> xa \<longleftrightarrow> x = 0) \<longleftrightarrow> xa = 1"
-proof auto
-  assume  1:"\<forall>x\<in>M. x \<in> xa \<longleftrightarrow> x = 0"
-  have "0\<in>xa" 
-    using 1 zero_in_M by simp
-  then show "xa=1" 
-    unfolding succ_def using equal_singleton[of _ xa 0] 
-              1 \<open>xa\<in>M\<close> trans_M Transset_intf[of M] by auto
-qed
-  *)
-end (* context forcing_data *)
-
-locale forces_rename = forcing_data + 
-  fixes fren :: "i" and fref :: "i" and auxren :: "i\<Rightarrow>i"
-  assumes
-  sats_fren: "[x,q,P,leq,one,p] @ env \<in> list(M) \<Longrightarrow> \<phi>\<in>formula \<Longrightarrow> 
-      sats(M, fren`\<phi>,[x,q,P,leq,one,p] @ env) \<longleftrightarrow> sats(M, \<phi>,[P,leq,one,q] @ env)"
-  and
-  arity_fren [simp]: "arity(fren`\<phi>) = arity(\<phi>) #+ 2"
-  and
-  sats_fref: "[x,P,leq,one,p] @ env \<in> list(M) \<Longrightarrow> \<phi>\<in>formula \<Longrightarrow> 
-      sats(M, fref`\<phi>,[x,P,leq,one,p] @ env) \<longleftrightarrow> sats(M, \<phi>,[P,leq,one,p,x] @ env)"
-  and
-  arity_fref [simp]: "arity(fref`\<phi>) = arity(\<phi>)"
-  and (* Note: this is a function i\<Rightarrow>i *)
-  sats_auxren: "[fec,tup,o,z,pp,l] @ env \<in> list(M) \<Longrightarrow> \<phi>\<in>formula \<Longrightarrow> 
-      sats(M,auxren(\<phi>),[fec,tup,o,z,pp,l] @ env) \<longleftrightarrow> sats(M,\<phi>,[pp,l,fec,tup,o,z] @ env)"
-  and
-  arity_auxren [simp]: "arity(auxren(\<phi>)) = arity(\<phi>)"
-  and
-  renaming_type [TC]: "\<phi>\<in>formula \<Longrightarrow> fren`\<phi> \<in> formula" "\<phi>\<in>formula \<Longrightarrow> fref`\<phi> \<in> formula"
-         "\<phi>\<in>formula \<Longrightarrow> auxren(\<phi>) \<in> formula"
-  and
-  wfrec_isHfrcat_replacement: "wfrec_replacement(##M, is_Hfrc_at(##M, P, leq), forcerel(fnnc)^+)"
-
-begin
+lemma sats_ren_forces_nand: 
+  "[q,P,leq,o,p] @ env \<in> list(M) \<Longrightarrow> \<phi>\<in>formula \<Longrightarrow> 
+   sats(M, ren_forces_nand(\<phi>),[q,P,leq,o,p] @ env) \<longleftrightarrow> sats(M, \<phi>,[P,leq,o,q] @ env)"
+  sorry
 
 definition
+  ren_forces_forall :: "i\<Rightarrow>i" where
+  "ren_forces_forall(f) \<equiv> f" 
+
+lemma ren_forces_forall_type[TC] :
+  "\<phi>\<in>formula \<Longrightarrow> ren_forces_forall(\<phi>) \<in>formula" 
+  unfolding ren_forces_forall_def by simp
+
+lemma sats_ren_forces_forall :
+  "[x,P,leq,one,p] @ env \<in> list(M) \<Longrightarrow> \<phi>\<in>formula \<Longrightarrow> 
+    sats(M, ren_forces_forall(\<phi>),[x,P,leq,o,p] @ env) \<longleftrightarrow> sats(M, \<phi>,[P,leq,o,p,x] @ env)"
+  sorry
+
+definition 
+  leq_fm :: "[i,i,i] \<Rightarrow> i" where
+  "leq_fm(leq,q,p) \<equiv> Exists(And(pair_fm(q#+1,p#+1,0),Member(0,leq#+1)))" 
+
+lemma leq_fm_type[TC] :
+  "\<lbrakk>leq\<in>nat;q\<in>nat;p\<in>nat\<rbrakk> \<Longrightarrow> leq_fm(leq,q,p)\<in>formula" 
+  unfolding leq_fm_def by simp
+
+lemma sats_leq_fm :
+  "\<lbrakk> leq\<in>nat;q\<in>nat;p\<in>nat;env\<in>list(A) \<rbrakk> \<Longrightarrow> 
+     sats(A,leq_fm(leq,q,p),env) \<longleftrightarrow> 
+    (\<exists>qp\<in>A. (pair(##A,nth(q,env),nth(p,env),qp) \<and>qp\<in>nth(leq,env)))" 
+  unfolding leq_fm_def by simp
+
+consts forces' :: "i\<Rightarrow>i"
+primrec
+  "forces'(Member(x,y)) = forces_mem_fm(0,1,3,x#+4,y#+4)"
+  "forces'(Equal(x,y))  = forces_eq_fm(0,1,3,x#+4,y#+4)"
+  "forces'(Nand(p,q))   = 
+        Neg(Exists(And(leq_fm(2,0,4),And(ren_forces_nand(forces'(p)),
+                                         ren_forces_nand(forces'(q))))))"
+  "forces'(Forall(p))   = Forall(ren_forces_forall(forces'(p)))" 
+
+definition 
   forces :: "i\<Rightarrow>i" where
-  "forces(\<phi>) \<equiv> And(Member(3,0),forces_ren(auxren,fren,fref, \<phi>))"
+  "forces(\<phi>) \<equiv> And(Member(3,0),forces'(\<phi>))"
 
-(*
-lemma sats_forces_eq_fm': 
-  assumes " [P,leq,one,p,t1,t2] @ env \<in> list(M)"
-  shows "sats(M,forces_eq_fm(auxren,0,1),[P,leq,one,p,t1,t2] @ env) \<longleftrightarrow>
-         sats(M,is_wfrec_fm(is_Hfrc_at_fm(5,6,2,1,0),2,3,4),
-       [P,leq,forcerel(<0,t1,t2,p>),<0,t1,t2,p>,1,0, one,p,t1,t2] @ env)"
-proof -
-  from assms
-  have "<0,t1,t2,p> \<in> M" 
-    using M_inhabit tuples_in_M by simp
-  then
-  have "forcerel(<0,t1,t2,p>) \<in> M" 
-    using forcerel_in_M by simp
-  note inM = assms oneN_in_M M_inhabit \<open><0,t1,t2,p>\<in>M\<close> \<open>forcerel(P,<0,t1,t2,p>)\<in>M\<close>
-  let ?\<phi>="is_wfrec_fm(is_Hfrc_at_fm(5,6,2,1,0),2,3,4)"
-  have "?\<phi>\<in>formula" unfolding is_Hfrc_at_fm_def by simp
-  let ?\<psi>="And(pair_fm(11,9,0),And(pair_fm(10,0,1),pair_fm(5,1,3)))"
-  let ?\<theta>="Exists(Exists(And(upair_fm(3,3,1),And(is_eclose_fm(1,0),is_frecrel_fm(0,2)))))"
-  from assms
-  have "sats(M,forces_eq_fm(auxren,0,1),[P,leq,one,p,t1,t2] @ env) \<longleftrightarrow> (\<exists>x\<in>M. \<exists>xa\<in>M. \<exists>xb\<in>M. \<exists>xc\<in>M.
-          sats(M,auxren(?\<phi>),[xc,xb,xa,x,P,leq,one,p,t1,t2] @ env) \<and>
-          xa = 1 \<and> sats(M,empty_fm(3),[xc,xb,1,x,P,leq,one,p,t1,t2] @ env) \<and>
-          sats(M,is_tuple_fm(3,8,9,7,1),[xc,xb,1,x,P,leq,one,p,t1,t2] @ env) \<and>
-          sats(M,?\<theta>,[xc,xb,1,x,P,leq,one,p,t1,t2] @ env))"
-    unfolding forces_eq_fm_def frecrel_eclose_fm_def
-    using M_inhabit def_one
-    by simp
-  moreover from assms
-  have "... \<longleftrightarrow> (\<exists>xa\<in>M. \<exists>xb\<in>M. \<exists>xc\<in>M.
-          sats(M,auxren(?\<phi>),[xc,xb,xa,0,P,leq,one,p,t1,t2] @ env) \<and>
-          xa = 1 \<and>
-          sats(M,is_tuple_fm(3,8,9,7,1),[xc,xb,1,0,P,leq,one,p,t1,t2] @ env) \<and>
-          sats(M,?\<theta>,[xc,xb,1,0,P,leq,one,p,t1,t2] @ env))"
-    using M_inhabit by force
-  moreover from assms
-  have " ... \<longleftrightarrow> (\<exists>xb\<in>M. \<exists>xc\<in>M.
-          sats(M,auxren(?\<phi>),[xc,xb,1,0,P,leq,one,p,t1,t2] @ env) \<and>
-          (\<exists>c1\<in>M. \<exists>c0\<in>M. sats(M,?\<psi>,[c0,c1,xc,xb,1,0,P,leq,one,p,t1,t2] @ env)) \<and>
-          sats(M,?\<theta>,[xc,xb,1,0,P,leq,one,p,t1,t2] @ env))"
-    using oneN_in_M M_inhabit unfolding is_tuple_fm_def by auto
-  moreover from assms
-  have " ... \<longleftrightarrow> (\<exists>xc\<in>M.
-          sats(M,auxren(?\<phi>),[xc,<0,t1,t2,p>,1,0,P,leq,one,p,t1,t2] @ env) \<and>
-          sats(M,?\<theta>,[xc,<0,t1,t2,p>,1,0,P,leq,one,p,t1,t2] @ env))"
-    using oneN_in_M M_inhabit tuples_in_M by auto
-  moreover from inM
-  have " ... \<longleftrightarrow> (\<exists>xc\<in>M.
-          sats(M,auxren(?\<phi>),[xc,<0,t1,t2,p>,1,0,P,leq,one,p,t1,t2] @ env) \<and>
-          (\<exists>s\<in>M. \<exists>ec\<in>M. sats(M,is_eclose_fm(1,0),[ec,s,xc,<0,t1,t2,p>,1,0,P,leq,one,p,t1,t2] @ env)
-               \<and>  sats(M,upair_fm(3,3,1),[ec,s,xc,<0,t1,t2,p>,1,0,P,leq,one,p,t1,t2] @ env)
-               \<and>  sats(M,is_frecrel_fm(0,2),[ec,s,xc,<0,t1,t2,p>,1,0,P,leq,one,p,t1,t2] @ env)) )"
-    by (simp)
-  moreover from inM
-  have " ... \<longleftrightarrow> sats(M,auxren(?\<phi>),[forcerel(P,<0,t1,t2,p>),<0,t1,t2,p>,1,0,P,leq,one,p,t1,t2] @ env)"
-    using sats_is_frecrel_fm[symmetric] cons_closed by simp
-  moreover from inM
-  have " ... \<longleftrightarrow> sats(M,?\<phi>,[P,leq,forcerel(P,<0,t1,t2,p>),<0,t1,t2,p>,1,0, one,p,t1,t2] @ env)"
-    using sats_auxren[OF _ \<open>?\<phi>\<in>formula\<close>, of _ _ _ _ _ _ "[one,p,t1,t2] @ env"] by (simp)
-  ultimately show ?thesis by simp
-qed
-*)
-
-
-lemma MH: "a0\<in>M \<Longrightarrow> a1\<in>M \<Longrightarrow> a2\<in>M \<Longrightarrow> a3\<in>M \<Longrightarrow> a4 \<in> M \<Longrightarrow> env\<in>list(M) \<Longrightarrow> 
-      is_Hfrc_at(##M,P,leq,a2,a1,a0) \<longleftrightarrow> sats(M,is_Hfrc_at_fm(5,6,2,1,0),[a0,a1,a2,a3,a4,P,leq] @ env)"
-  using sats_is_Hfrc_at_fm[of 5 6 2 1 0 "[a0,a1,a2,a3,a4,P,leq] @ env" M] P_in_M leq_in_M
-  by (simp)
-
-
-
-(*
-lemma sats_forces_eq_fm0: 
-  assumes  "p\<in>M" "t1\<in>M" "t2\<in>M" "env\<in>list(M)"
-  shows "sats(M,forces_eq_fm(auxren,0,1),[P,leq,one,p,t1,t2]@env) \<longleftrightarrow> is_frc_at(##M,P,leq,<0,t1,t2,p>,1)"
-proof -
-  have satsMH:"(is_Hfrc_at(##M, P, leq, a2, a1, a0) \<longleftrightarrow>
-        sats(M, is_Hfrc_at_fm(5, 6, 2, 1, 0),
-        [a0,a1,a2,a3,a4,P,leq,forcerel(P,<0,t1,t2,p>),<0,t1,t2,p>,1,0, one,p,t1,t2]@env))" 
-    if "a0\<in>M" "a1\<in>M" "a2\<in>M" "a3\<in>M" "a4\<in>M" for a0 a1 a2 a3 a4
-    using that assms P_in_M leq_in_M one_in_M 
-        sats_is_Hfrc_at_fm[of 5 6 2 1 0 
-        "[a0,a1,a2,a3,a4,P,leq,forcerel(P,<0,t1,t2,p>),<0,t1,t2,p>,1,0, one,p,t1,t2]@env"]
-        tuples_in_M zero_in_M oneN_in_M forcerel_in_M by simp
-  have "sats(M,is_wfrec_fm(is_Hfrc_at_fm(5,6,2,1,0),2,3,4),
-            [P,leq,forcerel(P,<0,t1,t2,p>),<0,t1,t2,p>,1,0, one,p,t1,t2]@env) \<longleftrightarrow>
-        is_frc_at(##M,P,leq,<0,t1,t2,p>,1)" 
-    unfolding is_frc_at_def using assms P_in_M leq_in_M one_in_M
-      forcerel_in_M tuples_in_M oneN_in_M zero_in_M sats_is_wfrec_fm[OF satsMH[simplified]]
-    by simp
-  then show ?thesis using assms P_in_M one_in_M leq_in_M sats_forces_eq_fm' by simp
-qed
-
-
-
-(* por qué tenemos el env? *)
-(*
-lemma sats_forces_eq_fm:
-  assumes  "[P,leq,one,p,t1,t2] @ env \<in> list(M)"
-  shows "sats(M,forces_eq_fm(auxren,0,1),[P,leq,one,p,t1,t2] @ env) \<longleftrightarrow> is_frc_at(##M,P,leq,<0,t1,t2,p>,1)"
-proof -
-  note assms
-  moreover from this
-  have "forcerel(P,\<langle>0, t1, t2, p\<rangle>)\<in>M" "\<langle>0, t1, t2, p\<rangle>\<in>M"
-    using tuples_in_M cons_closed eclose_closed M_inhabit forcerel_closed by simp_all
-  moreover from calculation
-  have "is_wfrec(##M,is_Hfrc_at(##M,P,leq),forcerel(P,\<langle>0,t1,t2,p\<rangle>),\<langle>0,t1,t2,p\<rangle>,1) \<longleftrightarrow>
-   is_wfrec(##M,\<lambda>x f z. z = bool_of_o(Hfrc(P,leq,x,f)),forcerel(P,\<langle>0,t1,t2,p\<rangle>),\<langle>0,t1,t2,p\<rangle>,1)"
-    using tuples_in_M oneN_in_M is_wfrec_cong[OF _ _ _ Hfrc_at_abs] (* esto es horrible *)
-    by simp
-  moreover from assms
-  have "Ord(length(env))" using nat_into_Ord[OF length_type, of env M] by simp
-  ultimately
-  show ?thesis
-  unfolding is_frc_at_def 
-  using forcerel_closed sats_forces_eq_fm' eclose_closed oneN_in_M M_inhabit tuples_in_M cons_closed
-    sats_is_wfrec_fm[OF MH[simplified], of "[forcerel(P,<0,t1,t2,p>), <0,t1,t2,p>, 1, 0, one, p, t1, t2] @ env" 2 3 4]
-     Hfrc_at_abs nat_into_Ord[OF length_type, of env M] by simp
-qed
-*)
-*)
-
-lemma forces_ren_type [TC]:  "\<phi>\<in>formula \<Longrightarrow> forces_ren(auxren,fren,fref, \<phi>) \<in> formula" 
+lemma forces'_type [TC]:  "\<phi>\<in>formula \<Longrightarrow> forces'(\<phi>) \<in> formula" 
   by (induct \<phi> set:formula; simp)
 
+lemma forces_type[TC] : "\<phi>\<in>formula \<Longrightarrow> forces(\<phi>) \<in> formula"
+  unfolding forces_def by simp
+
+lemma (in forcing_data) sats_forces_Member :
+  assumes  "x\<in>nat" "y\<in>nat" "env\<in>list(M)"
+           "nth(x,env)=xx" "nth(y,env)=yy" "q\<in>M" 
+         shows "sats(M,forces(Member(x,y)),[P,leq,one,q]@env) \<longleftrightarrow> 
+                (q\<in>P \<and> is_forces_mem(q,xx,yy))"
+  unfolding forces_def using assms sats_forces_mem_fm P_in_M leq_in_M one_in_M 
+  by simp
+
+lemma (in forcing_data) sats_forces_Equal :
+  assumes  "x\<in>nat" "y\<in>nat" "env\<in>list(M)"
+           "nth(x,env)=xx" "nth(y,env)=yy" "q\<in>M" 
+         shows "sats(M,forces(Equal(x,y)),[P,leq,one,q]@env) \<longleftrightarrow> 
+                (q\<in>P \<and> is_forces_eq(q,xx,yy))"
+  unfolding forces_def using assms sats_forces_eq_fm P_in_M leq_in_M one_in_M 
+  by simp
+
+lemma (in forcing_data) sats_forces_Nand :
+  assumes  "\<phi>\<in>formula" "\<psi>\<in>formula" "env\<in>list(M)" "p\<in>M" 
+  shows "sats(M,forces(Nand(\<phi>,\<psi>)),[P,leq,one,p]@env) \<longleftrightarrow> 
+         (p\<in>P \<and> \<not>(\<exists>q\<in>M. (\<exists>qp\<in>M. pair(##M,q,p,qp) \<and> qp\<in>leq) \<and> 
+               (sats(M,forces'(\<phi>),[P,leq,one,q]@env) \<and> sats(M,forces'(\<psi>),[P,leq,one,q]@env))))"
+  unfolding forces_def using sats_leq_fm assms sats_ren_forces_nand P_in_M leq_in_M one_in_M  
+  by simp
+  
+lemma (in forcing_data) sats_forces_Forall :
+  assumes  "\<phi>\<in>formula" "env\<in>list(M)" "p\<in>M" 
+  shows "sats(M,forces(Forall(\<phi>)),[P,leq,one,p]@env) \<longleftrightarrow> 
+         p\<in>P \<and> (\<forall>x\<in>M. sats(M,forces'(\<phi>),[P,leq,one,p,x]@env))"
+  unfolding forces_def using assms sats_ren_forces_forall P_in_M leq_in_M one_in_M  
+  by simp
+
+
+
+(*
 lemma arity_forces_ren:
   shows "\<phi>\<in>formula \<Longrightarrow> arity(forces_ren(auxren,fren,fref, \<phi>)) =  arity(\<phi>) #+ 4"
 proof (induct set:formula)
@@ -1285,102 +1150,6 @@ next
     apply (simp) (* This is false as it stands, it needs arity(\<phi>) \<noteq> 0 *)
     sorry
 qed
-
-lemma sats_forces_ren_Nand: 
-  assumes 
-    "[P,leq,one,p] @ env \<in> list(M)" "\<phi>\<in>formula" "\<psi>\<in>formula"
-  shows
-    "sats(M,forces_ren(auxren,fren,fref,Nand(\<phi>,\<psi>)),[P,leq,one,p] @ env) \<longleftrightarrow>
-          (\<forall>x\<in>M. x\<in>P \<longrightarrow> \<langle>x, p\<rangle> \<in> leq \<longrightarrow>
-          \<not> (sats(M, forces_ren(auxren,fren,fref,\<phi>),[P,leq,one,x] @ env) \<and>
-             sats(M, forces_ren(auxren,fren,fref,\<psi>),[P,leq,one,x] @ env)))"
-proof -
-  from assms
-  have "sats(M,forces_ren(auxren,fren,fref,Nand(\<phi>,\<psi>)),[P,leq,one,p] @ env) \<longleftrightarrow>
-          (\<forall>x\<in>M. x\<in>P \<longrightarrow> \<langle>x, p\<rangle> \<in> leq \<longrightarrow>
-          \<not> (sats(M, fren`forces_ren(auxren,fren,fref,\<phi>),[\<langle>x, p\<rangle>,x,P,leq,one,p] @ env) \<and>
-             sats(M, fren`forces_ren(auxren,fren,fref,\<psi>),[\<langle>x, p\<rangle>,x,P,leq,one,p] @ env)))"
-    using tuples_in_M  by simp
-  also from assms
-  have "... \<longleftrightarrow> (\<forall>x\<in>M. x\<in>P \<longrightarrow> \<langle>x, p\<rangle> \<in> leq \<longrightarrow>
-          \<not> (sats(M, forces_ren(auxren,fren,fref,\<phi>),[P,leq,one,x] @ env) \<and>
-             sats(M, forces_ren(auxren,fren,fref,\<psi>),[P,leq,one,x] @ env)))"
-    using tuples_in_M sats_fren by simp
-  finally
-  show ?thesis .
-qed
-
-lemma sats_forces_ren_Neg: "\<lbrakk> [P,leq,one,p] @ env \<in> list(M); \<phi>\<in>formula\<rbrakk> \<Longrightarrow>
-          sats(M,forces_ren(auxren,fren,fref,Neg(\<phi>)),[P,leq,one,p] @ env) \<longleftrightarrow> 
-          (\<forall>q\<in>M. q\<in>P \<longrightarrow> \<langle>q, p\<rangle> \<in> leq \<longrightarrow>
-          \<not> sats(M, forces_ren(auxren,fren,fref,\<phi>),[P,leq,one,q] @ env))" 
-  unfolding Neg_def sats_forces_ren_Nand
-  by simp
-
-lemma sats_forces_ren_Forall:
-  assumes
-    "p\<in>P" "[P,leq,one,p] @ env \<in> list(M)" "\<phi>\<in>formula"
-  shows
-    "sats(M,forces_ren(auxren,fren,fref,Forall(\<phi>)),[P,leq,one,p] @ env) \<longleftrightarrow> 
-     (\<forall>x\<in>M. sats(M, forces_ren(auxren,fren,fref,\<phi>),[P,leq,one,p,x] @ env))"
-  using assms sats_fref by simp
-
-lemma sats_forces_ren_Equal:
-  assumes
-    "p\<in>P" "[P,leq,one,p,x,y] @ env \<in> list(M)" 
-  shows
-    "sats(M,forces_ren(auxren,fren,fref,Equal(0,1)),[P,leq,one,p,x,y] @ env) \<longleftrightarrow> 
-     is_frc_at(<0,x,y,p>,1)"
-  using assms sats_forces_eq_fm[of 0 1 p x y] forcerel_in_M by simp
-
-lemma sats_forces_Nand: 
-  assumes 
-    "[P,leq,one,p] @ env \<in> list(M)" "\<phi>\<in>formula" "\<psi>\<in>formula" "p\<in>P"
-  shows
-    "sats(M,forces(Nand(\<phi>,\<psi>)),[P,leq,one,p] @ env) \<longleftrightarrow>
-          (\<forall>x\<in>M. x\<in>P \<longrightarrow> \<langle>x, p\<rangle> \<in> leq \<longrightarrow>
-          \<not> (sats(M, forces(\<phi>),[P,leq,one,x] @ env) \<and>
-             sats(M, forces(\<psi>),[P,leq,one,x] @ env)))" (is "?Q \<longleftrightarrow> _")
-  unfolding forces_def using sats_forces_ren_Nand assms by simp
-
-lemma sats_forces_Neg: "\<lbrakk> [P,leq,one,p] @ env \<in> list(M); \<phi>\<in>formula; p\<in>P\<rbrakk> \<Longrightarrow>
-          sats(M,forces(Neg(\<phi>)),[P,leq,one,p] @ env) \<longleftrightarrow> 
-          (\<forall>q\<in>M. q\<in>P \<longrightarrow> \<langle>q, p\<rangle> \<in> leq \<longrightarrow>
-          \<not> sats(M, forces(\<phi>),[P,leq,one,q] @ env))" 
-  unfolding forces_def using sats_forces_ren_Neg
-  by simp
-
-lemma sats_forces_Forall:
-  assumes
-    "p\<in>P" "env \<in> list(M)" "\<phi>\<in>formula"
-  shows
-    "sats(M,forces(Forall(\<phi>)),[P,leq,one,p] @ env) \<longleftrightarrow> 
-     (\<forall>x\<in>M. sats(M, forces(\<phi>),[P,leq,one,p,x] @ env))"
-  using assms sats_forces_ren_Forall P_in_M leq_in_M one_in_M
-    Transset_intf[OF trans_M _ P_in_M] unfolding forces_def by simp
-
-lemma sats_forces_Equal:
-  assumes
-    "p\<in>P" "x\<in>M" "y\<in>M" "env\<in>list(M)"
-  shows
-    "sats(M,forces(Equal(0,1)),[P,leq,one,p,x,y] @ env) \<longleftrightarrow> forces_eq(p,t1,t2) "
-  oops
-
-(*  using assms sats_forces_ren_Equal forcerel_in_M
-    wfrec_isHfrcat_replacement frc_at_abs  M_inhabit eclose_closed
-    tuples_in_M Transset_intf[OF trans_M _ P_in_M] oneN_in_M trancl_closed cons_closed
-  unfolding forces_def by simp
-*)
-lemma
-  assumes
-    "p\<in>P" "[P,leq,one,p] @ env \<in> list(M)" "\<phi>\<in>formula" "\<psi>\<in>formula"
-  shows
-    "sats(M,forces_ren(auxren,fren,fref,And(\<phi>,\<psi>)),[P,leq,one,p] @ env) \<longleftrightarrow>
-      sats(M, forces_ren(auxren,fren,fref,\<phi>),[P,leq,one,p] @ env) \<and>
-      sats(M, forces_ren(auxren,fren,fref,\<psi>),[P,leq,one,p] @ env)"
-  oops
-
-end (* forces_rename *)
 *)
 
-end
+end 
